Clean/Simplif.

transformations/Moore2Mealy/theorems/moore2mealy.v
@@ -9,168 +9,162 @@ Require Import List.
 Require Import Coq.Arith.EqNat.
 Require Import Bool.
 
-(** Moore machine *)
+(** * Moore machine *)
 
 (* Node: id x output *)
-Inductive N :=
-| n : nat -> nat -> N.
+Inductive Node :=
+ | node : nat -> nat -> Node.
 
-Definition N_id n0 := match n0 with n id o => id end. 
-Definition N_o n0 := match n0 with n id o => o end.
 Definition beq_N n1 n2 :=
-match n1, n2 with
-n id1 o1, n id2 o2 => beq_nat id1 id2 && beq_nat o1 o2
-end.
+  match n1, n2 with
+    node id1 o1, node id2 o2 => beq_nat id1 id2 && beq_nat o1 o2
+  end.
 
 (* Input pair: src node x input *)
 Inductive IPair :=
-| Ipr : N -> nat -> IPair.
+ | Ipr : Node -> nat -> IPair.
 
 Definition beq_IPair p1 p2 :=
-match p1, p2 with
-Ipr n1 i1, Ipr n2 i2 => beq_N n1 n2 && beq_nat i1 i2
-end.
+  match p1, p2 with
+    Ipr n1 i1, Ipr n2 i2 => beq_N n1 n2 && beq_nat i1 i2
+  end.
 
 (* Transition rule of moore machine: Input pair x trg node *)
 Inductive R :=
-| r : IPair -> N -> R.
-
-Definition R_Ip r0 := match r0 with r Ip0 n0 => Ip0 end. 
-Definition R_n r0 := match r0 with r Ip0 n0 => n0 end.
+ | r : IPair -> Node -> R.
 
 
 (* moore machine *)
 Definition P := list R.
 
 (* search output node in moore machine *)
-Fixpoint s (p: P) (Ip: IPair) : option N :=
-match p with
-| nil => None
-| r0 :: rs => 
-    if beq_IPair (R_Ip r0) Ip then 
-        Some (R_n r0) 
-    else 
-        s rs Ip 
-end.
+Fixpoint search (p: P) (i: IPair) : option Node :=
+  match p with
+  | nil => None
+  | (r a b) :: rs => 
+      if beq_IPair a i 
+      then 
+        Some b 
+      else 
+        search rs i 
+  end.
 
 (* semantics of moore machine  *)
-Fixpoint eval (p: P) (q0: N) (I: list nat) : list nat :=
-match I with 
-| nil => nil
-| i :: I' => 
-let input := (Ipr q0 i) in 
-    match (s p input) with
-    | None => nil
-    | Some oN => (N_o oN) :: eval p oN I'  
-    end
-end.
+Fixpoint eval (p: P) (q0: Node) (I: list nat) : list nat :=
+  match I with 
+  | nil => nil
+  | i :: I' => 
+      
+      match search p (Ipr q0 i) with
+      | None => nil (* error ? *)
+      | Some (node a b) => b :: eval p (node a b) I'  
+      end
+  end.
 
-(** Mealy machine *)
+(** * Mealy machine *)
 
 (* Output pair: trg node x output *)
 Inductive OPair :=
-| Opr : N -> nat -> OPair.
+ | Opr : Node -> nat -> OPair.
 
-Definition OPair_n Op0 := match Op0 with Opr n0 o0 => n0 end. 
-Definition OPair_o Op0 := match Op0 with Opr n0 o0 => o0 end.
 
 (* Transition rule of mealy machine : Input pair x trg node *)
 Inductive R' :=
-| r' : IPair -> OPair -> R'.
-
-Definition R'_Ip r0 := match r0 with r' Ip0 Op0 => Ip0 end. 
-Definition R'_Op r0 := match r0 with r' Ip0 Op0 => Op0 end.
+ | r' : IPair -> OPair -> R'.
 
 (* mealy machine *)
 Definition P' := list R'.
 
 (* search output node *)
-Fixpoint s' (p: P') (Ip: IPair) : option OPair :=
-match p with
-| nil => None
-| r0 :: rs => 
-    if beq_IPair (R'_Ip r0) Ip then 
-        Some (R'_Op r0) 
-    else 
-        s' rs Ip 
+Fixpoint search' (p: P') (i: IPair) : option OPair :=
+  match p with
+  | nil => None
+  | r' a b :: rs => 
+      if beq_IPair a i 
+      then 
+        Some b 
+      else 
+        search' rs i 
 end.
 
 (* semantics of mealy machine *)
-Fixpoint eval' (p: P') (q0: N) (I: list nat) : list nat :=
-match I with 
-| nil => nil
-| i :: I' => 
-let input := (Ipr q0 i) in 
-    match (s' p input) with
-    | None => nil
-    | Some oP => (OPair_o oP) :: eval' p (OPair_n oP) I'  
-    end
-end.
+Fixpoint eval' (p: P') (q0: Node) (I: list nat) : list nat :=
+  match I with 
+  | nil => nil
+  | i :: I' => 
+      match search' p (Ipr q0 i) with
+      | None => nil
+      | Some (Opr a b) => b :: eval' p a I'  
+      end
+  end.
 
-(** compiler *)
+(** * compiler *)
 
 (* compile moore to mealy *)
-Fixpoint compile (p: P) : P' :=
-match p with
-| nil => nil
-| rl :: rs => r' (R_Ip rl) (Opr (R_n rl) (N_o (R_n rl))) :: compile rs
-end.
+
+Definition compile_rule t := 
+  match t with 
+    r a (node c d) => r' a (Opr (node c d) d) 
+  end.
+
+Definition compile : P -> P' := List.map compile_rule.
 
 (* Lemma: when input pair is not matched by moore machine, 
    it is also not matched by the compiled mealy machine *)
 Lemma compile_s_correct_ca1:
-forall (p: P) (q0: N) (i: nat) (Ip: IPair),
-(Ipr q0 i) = Ip ->
-(s p Ip) = None ->
-(s' (compile p) Ip) = None.
+  forall (p: P) i,
+     search p i = None ->
+     search' (compile p) i = None.
 Proof.
-intros p q0 i Ip input s_of_P.
-induction p; simpl in s_of_P; simpl.
-- auto.
-- destruct (beq_IPair (R_Ip a) Ip).
-  + inversion s_of_P. 
-  + auto.
+  intros p i s_of_P.
+  induction p; simpl in s_of_P; simpl.
+  - reflexivity.
+  - destruct a. destruct n. simpl.
+    destruct (beq_IPair i0 i).
+    + discriminate s_of_P.
+    + auto.
 Qed.
+
+
 
 (* Lemma: when input pair is matched by moore machine, 
    it is also matched by the compiled mealy machine 
    their matched outputs are also a correspondence *)
 Lemma compile_s_correct_ca2:
-forall (p: P) (q0: N) (i: nat) (Ip: IPair) (n: N),
-(Ipr q0 i) = Ip ->
-(s p Ip) = Some n ->
-(s' (compile p) Ip) = Some (Opr n (N_o n)).
+  forall (p: P) i a b,
+    search p i = Some (node a b) ->
+    search' (compile p) i = Some (Opr (node a b) b).
 Proof.
-intros p q0 i Ip n input s_of_P.
-induction p; simpl in s_of_P; simpl.
-- inversion s_of_P.
-- destruct (beq_IPair (R_Ip a) Ip).
-  + inversion s_of_P as [id]. rewrite id. auto.
-  + auto.
+  intros p i a b s_of_P.
+  induction p; simpl in s_of_P; simpl.
+  - discriminate s_of_P.
+  - destruct a0. destruct n. simpl. 
+    destruct (beq_IPair i0 i).
+    + congruence. 
+    + auto.
 Qed.
 
 (* main theorem: compile is correct
    evaluation the same inputs produce the same output *)
 Theorem compile_correct:
-forall (p: P) (q0: N) (I: list nat),
+  forall (p: P) (q0: Node) (I: list nat),
     eval p q0 I = eval' (compile p) q0 I.
 Proof.
-intros p q0 I. revert q0.
-induction I as [|i].
-- (* I = nil *)
-  simpl. auto.  
-- (* I = i :: I /\ P(I') *) 
-  simpl. intro.
-  remember (Ipr q0 i) as input.
-  destruct (s p input) as [n|] eqn: s_of_P.
-  + (* input pair is matched by moore machine *)
-    assert ((s' (compile p) input) = Some (Opr n (N_o n))).
-    { specialize (compile_s_correct_ca2 p q0 i input). auto. }
-    rewrite H. simpl.
-    specialize (IHI n). rewrite IHI. auto.
-  + (* input pair is not matched by moore machine *)
-    assert ((s' (compile p) input) = None).
-    { specialize (compile_s_correct_ca1 p q0 i input). auto. }
-    rewrite H. auto.
+  intros p q0 I. revert q0.
+  induction I as [ | i I ].
+  - (* I = nil *)
+    intro ; reflexivity.
+  - (* I = i :: I /\ P(I') *) 
+    simpl. intro.
+    destruct (search p (Ipr q0 i)) as [ n | ] eqn: s_of_P.
+    + (* input pair is matched by moore machine *)
+      destruct n.
+      replace (search' (compile p) (Ipr q0 i)) with (Some (Opr (node n n0) n0)).
+      * f_equal ; auto.
+      * symmetry ; apply compile_s_correct_ca2. assumption. 
+    + (* input pair is not matched by moore machine *)
+      replace (search' (compile p) (Ipr q0 i)) with (@None OPair).
+      * reflexivity.
+      * symmetry ; apply compile_s_correct_ca1. assumption.
 Qed.
 
